code/experimental/ed25519/Hacl.Impl.Ed25519.PointDecompress.fst
@@ -1,0 +1,44 @@
+module Hacl.Impl.Ed25519.PointDecompress
+
+open FStar.Buffer
+open Hacl.UInt64
+open Hacl.Bignum25519
+open Hacl.Impl.Ed25519.ExtPoint
+
+
+val point_decompress:
+  out:Hacl.Impl.Ed25519.ExtPoint.point ->
+  s:buffer Hacl.UInt8.t{length s = 32} ->
+  Stack bool
+    (requires (fun h -> live h out /\ live h s))
+    (ensures (fun h0 b h1 -> live h0 s /\ live h1 out /\ modifies_1 out h0 h1))
+let point_decompress out s =
+  push_frame();
+  let tmp  = Buffer.create 0uL 10ul in
+  let y    = Buffer.sub tmp 0ul 5ul in
+  let x    = Buffer.sub tmp 5ul 5ul in
+  Hacl.Impl.Load51.load_51 y s;
+  let y0 = y.(0ul) in
+  let y1 = y.(1ul) in
+  let y2 = y.(2ul) in
+  let y3 = y.(3ul) in
+  let y4 = y.(4ul) in
+  let sign = (y4 >>^ 50ul) &^ 1uL in
+  let y4' = y4 &^ 0x7ffffffffffffuL in
+  Hacl.Lib.Create64.make_h64_5 y y0 y1 y2 y3 y4'; (* TODO: make sure that part is necessary *)
+  let z = Hacl.Impl.Ed25519.RecoverX.recover_x x y sign in
+  let res =
+  if z = false then false
+  else (
+    let outx = getx out in
+    let outy = gety out in
+    let outz = getz out in
+    let outt = gett out in
+    blit x 0ul outx 0ul 5ul;
+    blit y 0ul outy 0ul 5ul;
+    Hacl.Lib.Create64.make_h64_5 outz 1uL 0uL 0uL 0uL 0uL;
+    fmul outt x y;
+    true
+  ) in
+  pop_frame();
+  res
