code/experimental/ed25519/Hacl.Impl.Ed25519.Sign.fst
@@ -1,8 +1,10 @@
 module Hacl.Impl.Ed25519.Sign
 
 open FStar.Buffer
+open FStar.UInt32
 
 let hint8_p = buffer Hacl.UInt8.t
+
 
 val sign:
   signature:hint8_p{length signature = 64} ->
@@ -11,6 +13,51 @@ val sign:
   len:UInt32.t{UInt32.v len = length msg} ->
   Stack unit
     (requires (fun h -> live h signature /\ live h msg /\ live h secret))
-    (ensures (fun h0_ h1 -> live h0 secret /\ live h0 secret /\ live h1 signature /\ modifies_1 signature h0 h1))
+    (ensures (fun h0 _ h1 -> live h0 secret /\ live h0 secret /\ live h1 signature /\ modifies_1 signature h0 h1))
 let sign signature secret msg len =
-  
+  push_frame();
+  let tmp = create 0uL 40ul in
+  let g = Buffer.sub tmp 0ul 20ul in
+  let tmpa = Buffer.sub tmp 20ul 20ul in
+  Hacl.Impl.Ed25519.G.make_g g;
+  push_frame();
+  let buf = create 0uy 96ul in
+  let s' = Buffer.sub buf 0ul 64ul in
+  let a' = Buffer.create 0uL 5ul in
+  Hacl.Impl.Ed25519.SecretExpand.secret_expand s' secret;
+  let a = Buffer.sub s' 0ul 32ul in
+  let prefix = Buffer.sub s' 32ul 64ul in
+  Hacl.Impl.Ed25519.Ladder.point_mul tmpa a g;
+  Hacl.Impl.Ed25519.PointCompress.point_compress a' tmpa;
+  let a'' = create 0uy 32ul in
+  Hacl.Impl.Store51.store_51 a'' a';
+  let prefix_at_message = create 0uy (len +^ 64ul) in (* TODO: remove one copy of msg *)
+  blit prefix 0ul prefix_at_message 0ul 32ul;
+  blit msg 0ul prefix_at_message 32ul len;
+  let r = create 0uL 5ul in
+  Hacl.Impl.SHA512.ModQ.sha512_modq r prefix_at_message (len+^32ul);
+  let rb = create 0uy 32ul in
+  Hacl.Impl.Store51.store_51 rb r;
+  let r' = create 0uL 5ul in
+  Hacl.Impl.Ed25519.Ladder.point_mul r' rb g;
+  let rs = create 0uL 5ul in
+  Hacl.Impl.Ed25519.PointCompress.point_compress rs r';
+  let rs' = create 0uy 32ul in
+  Hacl.Impl.Store51.store_51 rs' rs;
+  let h = create 0uL 5ul in
+  blit rs'  0ul prefix_at_message 0ul 32ul;
+  blit a''  0ul prefix_at_message 32ul 32ul;
+  blit msg 0ul prefix_at_message 64ul len;
+  Hacl.Impl.SHA512.ModQ.sha512_modq h prefix_at_message (len+^64ul);
+  let aq = create 0uL 5ul in
+  Hacl.Impl.Load56.load_32_bytes aq a;
+  let ha = create 0uL 5ul in
+  Hacl.Impl.BignumQ.Mul.mul_modq ha h aq;
+  let s = create 0uL 5ul in
+  Hacl.Impl.BignumQ.Mul.add_modq s r ha;
+  let s' = create 0uy 32ul in
+  Hacl.Impl.Store56.store_56 s' s;
+  blit rs' 0ul signature 0ul 32ul;
+  blit s' 0ul signature 32ul 32ul;
+  pop_frame();
+  pop_frame()
