code/experimental/ed25519/Hacl.Impl.Load51.fst
@@ -1,0 +1,47 @@
+module Hacl.Impl.Load51
+
+open FStar.Mul
+open FStar.Buffer
+open FStar.Endianness
+
+open Hacl.Bignum.Parameters
+open Hacl.Spec.Bignum.Bigint
+open Hacl.Endianness
+open Hacl.UInt64
+
+let u32 = UInt32.t
+let h8 = Hacl.UInt8.t
+let h64 = Hacl.UInt64.t
+let hint8_p = buffer h8
+
+
+val load_51: output:felem -> input:hint8_p{length input = 32} -> Stack unit
+  (requires (fun h -> Buffer.live h output /\ Buffer.live h input))
+  (ensures (fun h0 _ h1 -> Buffer.live h0 output /\ Buffer.live h0 input
+    /\ Buffer.live h1 output /\ modifies_1 output h0 h1
+    /\ Hacl.Bignum25519.red_513 (as_seq h1 output)
+    (* /\ as_seq h1 output == Hacl.Spec.EC.Format.fexpand_spec (as_seq h0 input) *)))
+let load_51 output input =
+  let h = ST.get() in
+  Seq.lemma_eq_intro (Seq.slice (as_seq h input) 0 8) (as_seq h (Buffer.sub input 0ul 8ul));
+  Seq.lemma_eq_intro (Seq.slice (as_seq h input) 6 14) (as_seq h (Buffer.sub input 6ul 8ul));
+  Seq.lemma_eq_intro (Seq.slice (as_seq h input) 12 20) (as_seq h (Buffer.sub input 12ul 8ul));
+  Seq.lemma_eq_intro (Seq.slice (as_seq h input) 19 27) (as_seq h (Buffer.sub input 19ul 8ul));
+  Seq.lemma_eq_intro (Seq.slice (as_seq h input) 24 32) (as_seq h (Buffer.sub input 24ul 8ul));
+  let mask_51 = uint64_to_limb 0x7ffffffffffffuL in
+  let i0 = hload64_le (Buffer.sub input 0ul 8ul) in
+  let i1 = hload64_le (Buffer.sub input 6ul 8ul) in
+  let i2 = hload64_le (Buffer.sub input 12ul 8ul) in
+  let i3 = hload64_le (Buffer.sub input 19ul 8ul) in
+  let i4 = hload64_le (Buffer.sub input 24ul 8ul) in
+  let output0 = (i0         ) &^ mask_51 in
+  let output1 = (i1 >>^ 3ul ) &^ mask_51 in
+  let output2 = (i2 >>^ 6ul ) &^ mask_51 in
+  let output3 = (i3 >>^ 1ul ) &^ mask_51 in
+  let output4 = (i4 >>^ 12ul) &^ mask_51 in
+  UInt.logand_mask (v i0) (51);
+  UInt.logand_mask (v (i1 >>^ 3ul)) (51);
+  UInt.logand_mask (v (i2 >>^ 6ul )) (51);
+  UInt.logand_mask (v (i3 >>^ 1ul )) (51);
+  UInt.logand_mask (v (i4 >>^ 12ul)) (51);
+  Hacl.Lib.Create64.make_h64_5 output output0 output1 output2 output3 output4
